

$$\sim 1.3$$

a) $k+2 \quad 1$
 $i \geq n \quad 1$
 while $i > 0: n$
 $i = 1 \quad n+1$

$$T(n) = 1 + 1 + n + n + 1 = 3 + 2n$$

b) $i \geq n \quad 1$
 while $i > 1: (\log_2 n) + 1$
 $k+2 \quad \log_2 n$
 $i // 2 \quad \log_2 n$

$$\log_2 n = m$$

$$T(n) = 1 + \log_2 n + 1 + \log_2 n + \log_2 n = 2 + 3 \log_2 n = 2 + 3m$$

c) $i \geq 0 \quad 1$
 while $i < n: \frac{n}{2} + 1$
 $j \geq 0 \quad \frac{n}{2}$
 while $j < n: \frac{n}{2} \left(\frac{n}{2} + 1 \right)$
 $k+2 \quad \frac{n}{2}$
 $j \neq 2 \quad \frac{n^2}{4}$
 $i+2 \quad \frac{n}{2}$

$$T(n) = 1 + \frac{n}{2} + 1 + \frac{n}{2} + \frac{n^2}{4} + \frac{n}{2} + \frac{n^2}{4} + \frac{n^2}{2} + \frac{n}{2} = 2 + \frac{4n}{2} + \frac{3n^2}{2}$$

d) $i \geq 0 \quad 1$
 while $i < n: n+1$
 $j \geq 0 \quad n$
 while $j < i+1: \sum i^2 + n$
 $k+2 \quad (n-1)n(n+1)$
 $j \neq 1 \quad (n-1)n(n+1)$
 $i \neq 1 \quad n$

$$\sum_{i=0}^{n-1} i^2 = \frac{(n-1)n(n+1)}{6} = \int_0^n x^2 dx$$

$$T(n) = 1 + n + 1 + n + \sum + n + \sum + \sum + n = 2 + 4n + 3 \sum$$

e) $i \geq 1$
 while $i < n$:
 $j \geq 1$
 while $j < n$:
 $k \geq 1$
 $j = 2$
 $i = 2$

$\log_2 n + 1$
 $\log_2 n$
 $\log_2 n + (\log_2 n + 1)$
 $\log_2 n \log_2 n$
 $\log_2 n \log_2 n$
 $\log_2 n$

$$T(n) = 1 + \log_2 n + 1 + \log_2 n + 3 \log_2^2 n + \log_2 n = 2 + 3 \log_2 n + 4 \log_2^2 n$$

f) $i \geq 1$
 while $i < n$:
 $j \geq 1$
 while $j < n$:
 $k = 1$
 $j = 2$
 $i = 2$

$\log_2 n + 1$
 $\log_2 n$
 $\sum_{i=1}^n \log_2 \frac{n}{i} + 1$
 $\sum_{i=1}^n \log_2 \frac{n}{i}$
 $\log_2 n$

$$\sum_{i=1}^n \log_2 \frac{n}{i} = \log_2 n (\log_2 n + 1) = 5$$

$$\log_2 \frac{n}{i} = m$$

$$S = \frac{m(m+1)}{2}$$

$$T(n) = 1 + m + 1 + m + \frac{m(m+1)}{2} + m + \frac{m(m+1)}{2} + m = 2 + m(m+1) + 4m = 2 + m^2 + m + 4m = 2 + m^2 + 5m$$

~ 1.4

$$a) T(n) = \begin{cases} 1 & n \leq a, a > 0 \\ [T(n-a) + 1] & n > a \end{cases}$$

$$n > a \quad T(n) = T(n-a) + 1$$

$$\begin{aligned} T(n) &= [T(n-a) + 1] + 1 = T(n-2a) + 2 \\ &= [T(n-3a) + 1] + 2 = T(n-3a) + 3 = \dots \\ &= T(n-ma) + m \end{aligned}$$

$$n = ma + r \quad 0 \leq r < a$$

$$T(n) = T(r) + m$$

$$T(n) = m + 1, \quad r \leq a \quad T(r) = 1$$

$$m = \frac{n}{a} \quad T(n) = \frac{n}{a} + 1$$

$$b) T(n) = \begin{cases} 1 & n = 0 \\ [T(n-1) + d^n] & n \geq 1 \end{cases}$$

$$T(n) = [T(n-1) + d^{n+1}] + d^n = T(n-1) + d^{n+1} + d^n$$

$$T(n) = [T(n-2) + d^{n-1}] + d^{n-1} + d^n =$$

$$= T(n-2) + d^{n-1} + d^{n-1} + d^n$$

$$T(0) \quad T(n) = T(0) + d^1 + d^2 + \dots + d^n$$

$$\sum_{i=1}^n d^i = d^{n+1} - d$$

$$T(n) = 1 + (d^{n+1} - d) = d^{n+1} - 1$$

$$d(T/n) \approx \begin{cases} 1 & n=1 \\ \lfloor dT/\lfloor n/d \rfloor \rfloor + 1 & n \geq 2 \end{cases}$$

$$n \geq d^k \quad S(k) \approx T/d^k \quad S(0) \approx T/1 \approx 1$$

$$k \geq 1$$

$$S(k) \approx dS(k-1) + 1$$

$$S(k) \approx d[dS(k-2) + 1] + 1 \approx d^2 S(k-2) + d + 1$$

$$S(k) \approx d^2 [dS(k-3) + 1] + d + 1 \approx d^3 S(k-3) + d^2 + d + 1$$

~~...~~

$$S(k) \approx d^k S(0) + (d^{k-1} + d^{k-2} + \dots + d + 1)$$

$$d^{k-1} + d^{k-2} + \dots + 1 \approx d^k - 1$$

$$S(0) \approx 1$$

$$S(k) \approx d^k \cdot 1 + (d^k - 1) \approx d \cdot d^{k-1} \approx d^{k+1} - 1$$

$$n \geq d^k \Rightarrow k \approx \log_d n$$

$$T(n) \approx d^{\log_d n + 1} - 1 \approx d n - 1$$

$$d(T/n) \approx \begin{cases} 1 & n=1 \\ \lfloor aT/\lfloor n/a \rfloor \rfloor + n & n \geq 2, a \geq 2 \end{cases}$$

$$n \geq a^k \Rightarrow \lfloor \frac{n}{a^k} \rfloor \approx \frac{n}{a^k} \approx a^{k-1}$$

$$S(k) \approx T/a^k \Rightarrow S(0) \approx T/1 \approx 1$$

$$k \geq 1$$

$$S(k) \approx aS(k-1) + a^k$$

$$S(k) = a [a S(k-1) + a^{k-1}] + a^k$$

$$a^2 S(k-2) + a^k + a^k = a^2 S(k-2) + 2a^k$$

$$S(k) = a^2 [a S(k-3) + a^{k-2}] + 2a^k$$

$$2a^3S/(K-3) + a^k + 2a^k - a^3S/(K-3) + 3a^k$$

$$S(k) = a^k S(0) + k a^k = a^k + k a^k = a^k (1 + k)$$

$$n = a^k$$

$$K \approx \log_2 n$$

$$T(n) \leq n(\log_2 n + 1) \leq n \log_2 n + n$$